[OK] use inductive principle generated by Function

theories/check.v
@@ -13,26 +13,531 @@ OK, (r X \/ s X) => backchain for q X gives two solutions
 Is it important that the substitution in the Or note, X is a function?
 *)
 
-(* 
-  Given a checked program, and a deterministic tree,
-  then calling expand produces a tree which is still deterministic.
-*)
+
+Require Import FunInd.
+Functional Scheme expand_ind := Induction for expand Sort Prop.
+
+Definition sV_expand (S:sigV) Sexp:=
+  forall k, 
+    match lookup k Sexp with
+    | None => True
+    | Some Se =>
+      if lookup k S is Some S then incl Se S = ty_ok true
+      else forall (S':sigV), S' <> Sexp -> lookup k S' = None
+    end.
+
+Lemma sV_expand_refl {A}: sV_expand A A.
+Proof.
+  move=> //k.
+  case lookup => //= s.
+  rewrite incl_refl//.
+Qed.
+
 Lemma expand_det_tree {u sP sV sV' A r s ign d} : 
   check_program sP ->
     sigma2ctx sP s = Some sV ->
       det_tree_aux sP sV A ign = ty_ok (d, sV') ->
         expand u s A = r ->
           exists S d', minD d d' = d' /\ 
+          (* sV_expand sV' S /\ *)
+            det_tree_aux sP sV (get_tree r) d = ty_ok (d', S).
+Proof.
+  simpl in *.
+  move=> C.
+  move: sV sV' r d ign.
+  pattern u, s, A, (expand u s A).
+  apply: expand_ind; clear.
+  - move=> s []//= _ ???? _ _ [_ ->] <-/=; repeat eexists; rewrite ?minD_refl//.
+    (* apply: sV_expand_refl. *)
+  - move=> s []//= _ ???? _ _ [_ ->] <-/=; repeat eexists; rewrite ?minD_refl//.
+    (* apply: sV_expand_refl. *)
+  - move=> s []//= _ ???? _ _ [_ ->] <-/=; repeat eexists; rewrite ?minD_refl//.
+    (* apply: sV_expand_refl. *)
+  - admit.
+  - move=> s []//= _ ???? _ _ [_ ->] <-/=; repeat eexists; rewrite ?minD_refl//.
+    (* apply: sV_expand_refl. *)
+  - move=> s INIT A sB B HINIT dA IH sV sV' r d ign H/=.
+    rewrite is_dead_next_alt//= => dtB<-{r}.
+    have ?: sB = s by admit.
+    subst.
+    have:= IH _ _ _ _ _ _ _ erefl.
+    move=> /(_ _ _ _ _ H dtB).
+    move=> [S[d' [H1 H2]]].
+    rewrite get_tree_Or/= is_dead_next_alt//= H2.
+    by repeat eexists; eauto.
+  - move=> s INIT A sB B HINIT dA IH A' eA sV sV' r d ign H/=.
+    have fA:= expand_not_failed _ eA notF.
+    rewrite next_alt_not_failed//=.
+    move=> + <-{r}/=.
+    case nB: next_alt => [B'|]//=.
+      case dtA: (det_tree_aux _ _ A) => /=[[DA' sVA]|]//=.
+      case dtB: (det_tree_aux _ _ B) => /=[[DB sVB]|]//=.
+      case M: merge_sig => //=[S']; subst.
+      have {IH}/=[S[d'[H1 H2]]]:= IH _ _ _ _ _ H dtA eA.
+      move=> [??]; subst.
+      case nA: next_alt => [A''|]//=; last first.
+        have:= same_ty_det_tree_aux sP sV B ign (if has_cut A then maxD DA' DB else Pred).
+        rewrite dtB/=; case dtB': det_tree_aux => //=[[D' sVx]] /eqP[?]; subst sVx.
+        repeat eexists.
+        move: dtB'.
+        case: ifP => //=cA.
+        case N: maxD => //=.
+        destruct DA', DB => //=.
+        have [[] [//= _ {}H]] := det_tree_aux_func2 dtB.
+        rewrite H; congruence.
+      have:= same_ty_det_tree_aux sP sV A' DA'(if has_cut A then maxD DA' DB else Pred).
+      rewrite H2; case dtA' : det_tree_aux => //=[[Dx Sx]] /eqP[?]; subst Sx.
+      have:= same_ty_det_tree_aux sP sV B ign (if has_cut A then maxD DA' DB else Pred).
+      rewrite dtB/=; case dtB': det_tree_aux => //=[[Dy Sy]] /eqP[?]; subst Sy.
+      case M1: merge_sig => /=[S'|].
+        repeat eexists.
+        move: dtB' dtA'.
+        case: ifP => cA//.
+        destruct DA' => //=.
+        destruct DB => //=.
+        rewrite H2 => +[?]; subst.
+        have [[][//_ Hz]] := det_tree_aux_func2 dtB.
+        rewrite Hz => -[?]; subst; rewrite maxD_comm/=.
+        simpl in H1; subst.
+        rewrite (expand_Exp_has_cut _ eA)//=.
+      (* BELOW: SHOULD NOT BE REACHABLE: merge_sig S sVB is a ty_ok *)
+      (* sV1 <= sVA
+          sV1 <= sVB
+          sVA + sVB = sV2
+          sV1 <= S 
+          ==========> 
+          goal: merge_sig S sVB = ty_ok
+          IDEA: all vars in S have "compatible" with sVA
+          and all variables not appearing in sVA are also not in sVB, i.e. they are fresh
+
+          FORMALLY:
+          forall x \in S, if x \in sVA, then they are compatible,
+                          else x is not in sVB
+      *)
+      idtac.
+      admit.
+    move=> H2.
+    have /=[S[d' [H3 H4]]]  := IH _ _ _ _ _ H H2 eA.
+    rewrite H4/=.
+    have /= [d1[MM ->]]:= next_alt_None_dt sP sV d nB.
+    case: eqP => Hz; repeat eexists; auto.
+  - move=> s INIT A sB B HINIT dA IH A' eA sV sV' r d ign H/=.
+    have fA:= expand_not_failed _ eA notF.
+    rewrite next_alt_not_failed//=.
+    move=> + <-{r}/=.
+    rewrite (is_ko_det_tree_aux is_ko_cutr)/=(is_ko_next_alt _ is_ko_cutr)/=.
+    case nB: next_alt => [B'|]//=.
+      case dtA: (det_tree_aux _ _ A) => /=[[DA' sVA]|]//=.
+      case dtB: (det_tree_aux _ _ B) => /=[[DB sVB]|]//=.
+      case M: merge_sig => //=[S']; subst.
+      move=> [??]; subst.
+      have /=[S[d' [H1 H2]]] := IH _ _ _ _ _ H dtA eA.
+      have := same_ty_det_tree_aux sP sV A' DA' (if has_cut A then maxD DA' DB else Pred).
+      rewrite H2/= => /eqP.
+      case Hz : det_tree_aux => //=[[Dx sX]][?]; subst sX.
+      case: eqP; repeat eexists; rewrite //=?minD_refl//=.
+      move: Hz.
+      case:ifP => //= cA.
+      destruct DA'; simpl in *; subst => //.
+      destruct DB => //=; congruence.
+    move=> H2.
+    have /=[S[d' [H0 H1]]]  := IH _ _ _ _ _ H H2 eA.
+    rewrite H1/=.
+    by case:ifP => //=; repeat eexists; auto; rewrite minD_refl.
+  - move=> s INIT A sB B HINIT dA IH A' eA sV sV' r d ign H/=.
+    have [? fA] := expand_failed_same _ eA; subst A'.
+    move=> +<-{r}/=.
+    case nA: next_alt => [A'|]//=; last first.
+      move=> H2.
+      have := same_ty_det_tree_aux sP sV B ign d.
+      rewrite H2/=; case H3: det_tree_aux => /=[[D1 Sx]|] => //=/eqP[?]; subst Sx.
+      repeat eexists.
+      destruct d => //=.
+      have [d2[H4 H5]]:= det_tree_aux_func2 H2.
+      destruct d2 => //=.
+      congruence.
+    case nB: next_alt => [B'|]//=; last first.
+      move=> H2.
+      have [d2[H3 H4]]:= det_tree_aux_func2 H2.
+      rewrite minD_comm in H3.
+      destruct d; simpl in H3; subst.
+        by rewrite H4; repeat eexists.
+      move=>/=.
+      have := same_ty_det_tree_aux sP sV A ign Pred.
+      by rewrite H2/=; case: det_tree_aux => //= -[]//=; repeat eexists.
+    case dtA: (det_tree_aux _ _ A) => /=[[DA' sVA]|]//=.
+    case dtB: (det_tree_aux _ _ B) => /=[[DB sVB]|]//=.
+    case M: merge_sig => //=[S'][??]; subst.
+    pose X := if has_cut A then maxD DA' DB else Pred.
+    rewrite -/X.
+    have := same_ty_det_tree_aux sP sV A ign X.
+    rewrite dtA; case dtA': det_tree_aux => //=[[d' blah]]/eqP[?]; subst blah.
+    have := same_ty_det_tree_aux sP sV B ign X.
+    rewrite dtB; case dtB': det_tree_aux => //=[[d1 blah]]/eqP[?]; subst blah.
+    rewrite M/=; repeat eexists.
+    move: dtA' dtB'; rewrite/X.
+    case:ifP => // c.
+    destruct DA' => //=.
+    destruct DB => //=.
+    have [[][//_ ->]] := det_tree_aux_func2 dtA.
+    move=> [?]; subst => /=.
+    have [[][//_ ->]] := det_tree_aux_func2 dtB; congruence.
+  - move=> s INIT A sB B HINIT dA IH A' eA sV sV' r d ign H/=.
+    have [? sA]:= expand_solved_same _ eA; subst A'.
+    move=> +<-{r}/=.
+    rewrite next_alt_not_failed?success_failed//=.
+    case nB: next_alt => [B'|]//=; last first.
+      move=> H2; have [d2[H3 H4]] := det_tree_aux_func2 H2.
+      have := same_ty_det_tree_aux sP sV A ign d.
+      rewrite H2; case dtA': det_tree_aux => //=[[d' blah]]/eqP[?]; subst blah.
+      repeat eexists; destruct d2; simpl in H3; subst => //.
+      destruct d => //=; congruence.
+    case dtA: (det_tree_aux _ _ A) => /=[[DA' sVA]|]//=.
+    case dtB: (det_tree_aux _ _ B) => /=[[DB sVB]|]//=.
+    case M: merge_sig => //=[S'][??]; subst.
+    have [d2[H2 H3]] := det_tree_aux_func2 dtB.
+    have [d3[H4 H5]]:= det_tree_aux_func2 dtA.
+    pose X := if has_cut A then maxD DA' DB else Pred.
+    rewrite -/X.
+    have := same_ty_det_tree_aux sP sV A ign X.
+    rewrite dtA; case dtA': det_tree_aux => //=[[d' blah]]/eqP[?]; subst blah.
+    have := same_ty_det_tree_aux sP sV B ign X.
+    rewrite dtB; case dtB': det_tree_aux => //=[[d1 blah]]/eqP[?]; subst blah.
+    rewrite M/=; repeat eexists.
+    move: dtA' dtB'; rewrite/X.
+    case:ifP => // c.
+    destruct DA' => //=.
+    destruct DB => //=.
+    have [[][//_ ->]] := det_tree_aux_func2 dtA.
+    move=> [?]; subst => /=.
+    have [[][//_ ->]] := det_tree_aux_func2 dtB; congruence.
+  - move=> s INIT A B0 B HINIT IH A' eA sV sV' r d ign H/=.
+    have fA:= expand_not_failed _ eA notF.
+    have sA:= expand_not_solved_not_success _ eA notF.
+    rewrite fA (next_alt_not_failed fA)//= sA/=.
+    move=> + <-{r}/=.
+    case nB0: next_alt => [B0'|]//=.
+      case dtA: (det_tree_aux _ _ A) => /=[[DA' sVA]|]//=.
+      case dtB0: (det_tree_aux _ _ B0) => /=[[DB0 sVB0]|]//=.
+      case dtB: (det_tree_aux _ _ B) => /=[[DB sVB]|]//=.
+      case M: merge_sig => //=[S'][??]; subst.
+      rewrite orbF andbF/=.
+      have {IH}/=[S[d'[H4 H5]]] := IH _ _ _ _ _ H dtA eA.
+      case nA: next_alt => [A''|]//=; last first.
+        repeat eexists; rewrite minD_refl//.
+      have [d0[//H2 H3]] := det_tree_aux_func2 dtB.
+      case: ifP => fA'.
+        have := same_ty_det_tree_aux sP sV A' DA' (maxD DB0 DB).
+        rewrite H5; case dtA': det_tree_aux => //=[[d2 blah]]/eqP[?]; subst blah.
+        (* in S there are more assignemnts than in sV *)
+        (* all of this new assigments will never appear in B0
+            all output are the same more precise
+        *)
+        admit. (*PB WITH SIG*)
+      rewrite orbF.
+      case: ifP.
+        move=> /andP[sA' /eqP nA'].
+        have [dd[//H6 H7]] := next_alt_None_dt sP sV (maxD DB0 DB) nA'.
+        rewrite H7/=.
+        case nB: next_alt => [B'|]//=; last first.
+          by repeat eexists; rewrite minD_refl.
+        (* (DEAD \/ (OK /\ ... ! /\ ... OK) \/ Any) /\ B  -> OK /\ B *)
+        admit. (*PB WITH SIG*)
+      have := same_ty_det_tree_aux sP sV A' DA' (maxD DB0 DB).
+      rewrite H5; case dtA': det_tree_aux => //=[[d2 blah]]/eqP[?]; subst blah.
+      case sA' : success => //=.
+        move=> {nA A''}.
+        case nA: next_alt => [A''|]//= _.
+        admit. (*PB WITH SIG*)
+      move=> _.
+      admit. (*PB WITH SIG*)
+    case nB: next_alt => [B'|]//=.
+      case dtA: (det_tree_aux _ _ A) => /=[[DA' sVA]|]//=.
+      case dtB0: (det_tree_aux _ _ B0) => /=[[DB0 sVB0]|]//=.
+      case dtB: (det_tree_aux _ _ B) => /=[[DB sVB]|]//=.
+      case M: merge_sig => //=[S'][??]; subst.
+      rewrite orbF andbT.
+      case nA: next_alt => [A''|]//=; last first; rewrite?orbF?orbT/=.
+        repeat eexists; rewrite minD_refl//.
+      rewrite andbT.
+      case: ifP => fA'.
+        repeat eexists; rewrite minD_refl//.
+      rewrite fA'.
+      have [dd[//H2 H3]] := det_tree_aux_func2 dtB.
+      have [d2[H4 H5]] := det_tree_aux_func2 dtA.
+      have {IH}/=[S[d'[H6 H7]]] := IH _ _ _ _ _ H dtA eA.
+      have := same_ty_det_tree_aux sP sV A' DA' (maxD DB0 DB).
+      rewrite H7; case dtA': det_tree_aux => //=[[d3 blah]]/eqP[?]; subst blah.
+      case: ifP => sA'.
+        admit. (*PB WITH SIG*)
+      admit. (*PB WITH SIG*)
+    move=> [??]; subst.
+    rewrite andbT orbT; repeat eexists; rewrite minD_refl//.
+  - move=> s INIT A B0 B HINIT IH A' eA sV sV' r d ign H/=.
+    have fA:= expand_not_failed _ eA notF.
+    have sA:= expand_not_solved_not_success _ eA notF.
+    rewrite fA (next_alt_not_failed fA)//= sA/= => +<-{r}/=.
+    case nB0: next_alt => [B0'|]//=.
+      case dtA: (det_tree_aux _ _ A) => /=[[DA' sVA]|]//=.
+      case dtB0: (det_tree_aux _ _ B0) => /=[[DB0 sVB0]|]//=.
+      case dtB: (det_tree_aux _ _ B) => /=[[DB sVB]|]//=.
+      case M: merge_sig => //=[S'][??]; subst.
+      rewrite orbF andbF/=.
+      case nA: next_alt => [A''|]//=; last first.
+        by repeat eexists; rewrite minD_refl.
+      have [xx[//H2 H3]] := det_tree_aux_func2 dtB.
+      have /=[S[d'[H4 H5]]] := IH _ _ _ _ _ H dtA eA.
+      have := same_ty_det_tree_aux sP sV A' DA' (maxD DB0 DB).
+      rewrite H5; case dtA': det_tree_aux => //=[[d2 blah]]/eqP[?]; subst blah.
+      case: ifP => fA'.
+        admit. (*PB WITH SIG*)
+      rewrite orbF/=.
+      case:ifP => H1/=.
+        case:ifP.
+          repeat eexists; rewrite minD_refl//.
+        move=> /eqP nB.
+        admit. (*PB WITH SIG*)
+      admit. (*PB WITH SIG*)
+    rewrite !orbT/=!andbT/=.
+    case nB: next_alt => [B'|]//=; rewrite?orbF ?orbT/=; last first.
+      by move=> [??]; subst; repeat eexists; rewrite minD_refl.
+    case dtA: (det_tree_aux _ _ A) => /=[[DA' sVA]|]//=.
+    case dtB0: (det_tree_aux _ _ B0) => /=[[DB0 sVB0]|]//=.
+    case dtB: (det_tree_aux _ _ B) => /=[[DB sVB]|]//=.
+    case M: merge_sig => //=[S'][??]; subst.
+    case fA': failed => /=.
+      repeat eexists.
+      by rewrite minD_refl.
+    rewrite next_alt_not_failed//=.
+    case:ifP => sA'.
+      admit. (*PB WITH SIG*)
+    have /=[S[d'[H4 H5]]] := IH _ _ _ _ _ H dtA eA.
+    have := same_ty_det_tree_aux sP sV A' DA' (maxD DB0 DB).
+    rewrite H5; case dtA': det_tree_aux => //=[[d2 blah]]/eqP[?]; subst blah.
+    admit. (*PB WITH SIG*)
+  - move=> s INIT A B0 B HINIT IH A' eA sV sV' r d ign H/=.
+    have [? fA]:= expand_failed_same _ eA; subst A' => +<-{r}/=.
+    rewrite fA/=.
+    case:ifP => H1.
+      move=> [??]; subst.
+      by repeat eexists; rewrite minD_refl.
+    case dtA: (det_tree_aux _ _ A) => /=[[DA' sVA]|]//= dtB0.
+    have:= same_ty_det_tree_aux sP sV A ign d.
+    rewrite dtA; case dtA' : det_tree_aux => /=[[DA'' blah]|]//=/eqP[?]; subst blah.
+    have:= same_ty_det_tree_aux sP sVA B0 DA' DA''.
+    rewrite dtB0; case dtB0' : det_tree_aux => /=[[DB0'' blah]|]//=/eqP[?]; subst blah.
+    repeat eexists.
+    destruct d => //=.
+    move: H1.
+    case nB0: next_alt => [B0'|]//=; rewrite orbF.
+    case nA: next_alt => [A'|]//= _.
+    have /=[S[d'[H4 H5]]] := IH _ _ _ _ _ H dtA eA.
+    destruct DA'; destruct DA''; simpl in H4; try congruence.
+    have [[][//_]] := det_tree_aux_func2 dtB0; congruence.
+  - move=> s INIT A B0 B HINIT HL A' eA HR sV sV' r d ign H/=.
+    have [? sA]:= expand_solved_same _ eA; subst A'.
+    have fA:= success_failed _ sA.
+    rewrite sA fA (next_alt_not_failed fA)/=.
+    case e1: expand => //=[B'|B'|B'|B'].
+    - have fB:= expand_not_failed _ e1 notF.
+      have sB:= expand_not_solved_not_success _ e1 notF.
+      rewrite (next_alt_not_failed fB)//= andbF/=.
+      move=> + <-{r}/=; rewrite fA sA/= (next_alt_not_failed fA)/=.
+      case nA: next_alt => [A'|]//=.
+        case nB0: next_alt => [B0'|]//=.
+          case dtA: (det_tree_aux _ _ A) => /=[[DA' sVA]|]//=.
+          case dtB0: (det_tree_aux _ _ B0) => /=[[DB0 sVB0]|]//=.
+          case dtB: (det_tree_aux _ _ B) => /=[[DB sVB]|]//=.
+          case M: merge_sig => //=[S'][??]; subst.
+          have := same_ty_det_tree_aux sP sV A ign (maxD DB0 DB).
+          rewrite dtA; case dtA': det_tree_aux => //=[[d2 blah]]/eqP[?]; subst blah.
+          
+          have := same_ty_det_tree_aux sP sVA B0 DA' d2.
+          rewrite dtB0; case dtB0': det_tree_aux => //=[[d3 blah]]/eqP[?]; subst blah.
+
+          have /= := HR _ _ _ _ _ _ dtB e1.
+          (*PB WITH IH*)
+          admit.
+        move=> dtB.
+        case nB: next_alt => [B''|]//=.
+          apply: HR _ _ _ _ _ _ dtB e1.
+          admit. (*PB WITH IH*)
+        repeat eexists; rewrite minD_refl//.
+      case nB0: next_alt => [B0'|]//=.
+        case dtA: (det_tree_aux _ _ A) => /=[[DA' sVA]|]//=dtB.
+        have := same_ty_det_tree_aux sP sV A ign d.
+        rewrite dtA; case dtA': det_tree_aux => //=[[d2 blah]]/eqP[?]; subst blah.
+        case:eqP => nB'.
+          by repeat eexists; rewrite minD_refl.
+        admit.
+      move=> dtB.
+      case nB: next_alt => [B''|]//=.
+        apply: HR dtB e1.
+        admit.
+      repeat eexists; rewrite minD_refl//.
+    - have fB:= expand_not_failed _ e1 notF.
+      have sB:= expand_not_solved_not_success _ e1 notF.
+      rewrite (next_alt_not_failed fB)//= andbF/=.
+      move=> + <-{r}/=.
+      rewrite (is_ko_next_alt _ is_ko_cutr)/=.
+      rewrite failed_success_cut success_cut sA/=next_alt_cutl/=.
+      rewrite (@next_alt_not_failed (cutl A))/=; last first.
+        rewrite failed_success_cut success_cut sA//.
+      case nA: next_alt => [A'|]//=.
+        case nB0: next_alt => [B0'|]//=.
+          case dtA: (det_tree_aux _ _ A) => /=[[DA' sVA]|]//=.
+          case dtB0: (det_tree_aux _ _ B0) => /=[[DB0 sVB0]|]//=.
+          case dtB: (det_tree_aux _ _ B) => /=[[DB sVB]|]//=.
+          case M: merge_sig => //=[S'][??]; subst.
+          case: eqP => nB'.
+            by repeat eexists; rewrite minD_refl//.
+          admit.
+        move=> H1.
+        case nB: next_alt => [B''|]/=; last first.
+          by repeat eexists; rewrite minD_refl.
+        apply: HR _ _ _ _ _ _ H1 e1.
+        admit.
+      case nB0: next_alt => [B0'|]//=.
+        case dtA: (det_tree_aux _ _ A) => /=[[DA' sVA]|]//=.
+        case dtB: (det_tree_aux _ _ B) => /=[[DB sVB]|]//=[??]; subst.
+        case nB: next_alt => [B''|]/=; last first.
+          by repeat eexists; rewrite minD_refl.
+        have [d1[H1]] := next_alt_None_dt sP sV ign nA.
+        rewrite dtA => -[??]; subst.
+        apply: HR dtB e1.
+        admit.
+      move=> dtB.
+      case nB: next_alt => [B''|]/=; last first.
+        by repeat eexists; rewrite minD_refl.
+      apply: HR dtB e1.
+      admit.
+    - have [? fB]:= expand_failed_same _ e1; subst B' => +<-{r}/=.
+      rewrite fA/=sA (next_alt_not_failed fA)/=.
+      case nB0: (next_alt _ B0) => [B0'|]//=.
+        rewrite orbF/=.
+        case nA: next_alt => [A'|]//=.
+          case dtA: (det_tree_aux _ _ A) => /=[[DA' sVA]|]//=.
+          case dtB0: (det_tree_aux _ _ B0) => /=[[DB0 sVB0]|]//=.
+          case dtB: (det_tree_aux _ _ B) => /=[[DB sVB]|]//=.
+          case M: merge_sig => //=[S'][??]; subst.
+          have := same_ty_det_tree_aux sP sV A ign (maxD DB0 DB).
+          rewrite dtA; case dtA': det_tree_aux => //=[[d2 blah]]/eqP[?]; subst blah.
+          have := same_ty_det_tree_aux sP sVA B DA' d2.
+          rewrite dtB; case dtB': det_tree_aux => //=[[d3 blah]]/eqP[?]; subst blah.
+          have := same_ty_det_tree_aux sP sVA B0 DA' d2.
+          rewrite dtB0; case dtB0': det_tree_aux => //=[[d4 blah]]/eqP[?]; subst blah.
+          rewrite M/=.
+          repeat eexists.
+          destruct DB0, DB => //=; simpl in *.
+          have /=[Sx [d'[H1 H2]]] := HL _ _ _ _ _ H dtA eA.
+          admit.
+        case nB: next_alt => [B''|]//=.
+          case dtA: (det_tree_aux _ _ A) => /=[[DA' sVA]|]//=.
+          move=>dtB.
+          have := same_ty_det_tree_aux sP sV A ign d.
+          rewrite dtA; case dtA': det_tree_aux => //=[[d2 blah]]/eqP[?]; subst blah.
+          have := same_ty_det_tree_aux sP sVA B DA' d2.
+          rewrite dtB; case dtB': det_tree_aux => //=[[d3 blah]]/eqP[?]; subst blah.
+          repeat eexists.
+          have /=[Sx [d'[H1 H2]]] := HL _ _ _ _ _ H dtA eA.
+          destruct d => //=.
+          admit.
+        move=> [??]; subst.
+        by repeat eexists; rewrite minD_refl.
+      case nB: next_alt => [B'|]//=; last first.
+        move=> [??]; subst.
+        by repeat eexists; rewrite minD_refl.
+      rewrite orbT/= => dtB.
+      have:= same_ty_det_tree_aux sP sV B ign d.
+      rewrite dtB; case dtB' : det_tree_aux => /=[[DB' blah]|]//=/eqP[?]; subst blah.
+      repeat eexists.
+      destruct d => //=.
+      have [[][//_ ]] := det_tree_aux_func2 dtB.
+      congruence.
+    - have [? sB]:= expand_solved_same _ e1; subst B'.
+      have fB:= success_failed _ sB.
+      move=> +<-{r}/=; rewrite fA sA /=.
+      rewrite (next_alt_not_failed fB) andbF/=.
+      rewrite (next_alt_not_failed fA)/=.
+      case nA: next_alt => [A'|]//=.
+        case nB0: (next_alt _ B0) => [B0'|]//=.
+          case dtA: (det_tree_aux _ _ A) => /=[[DA' sVA]|]//=.
+          case dtB0: (det_tree_aux _ _ B0) => /=[[DB0 sVB0]|]//=.
+          case dtB: (det_tree_aux _ _ B) => /=[[DB sVB]|]//=.
+          case M: merge_sig => //=[S'][??]; subst.
+          have /=[Sx [d'[H1 H2]]] := HL _ _ _ _ _ H dtA eA.
+          (* have /= := HR _ _ _ _ _ _ _ dtB e1. *)
+          have:= same_ty_det_tree_aux sP sV A ign (maxD DB0 DB).
+          rewrite dtA; case dtA' : det_tree_aux => /=[[DA'' blah]|]//=/eqP[?]; subst blah.
+          have:= same_ty_det_tree_aux sP sVA B0 DA' DA''.
+          rewrite dtB0; case dtB0' : det_tree_aux => /=[[DB0'' blah]|]//=/eqP[?]; subst blah.
+          have:= same_ty_det_tree_aux sP sVA B DA' DA''.
+          rewrite dtB; case dtB' : det_tree_aux => /=[[DB'' blah]|]//=/eqP[?]; subst blah.
+          rewrite M/=.
+          repeat eexists.
+          destruct DB0 => //=.
+          destruct DB => //=.
+          simpl in *.
+          have [[][//_ H3]] := det_tree_aux_func2 dtB0.
+          have [[][//_ H4]] := det_tree_aux_func2 dtB.
+          destruct DA''.
+            have->/=: DB0'' = Func by congruence.
+            by have->/=: DB'' = Func by congruence.
+          destruct DA'; simpl in H1; subst => //=; try congruence.
+          admit. (*PB with max DB0 DB*)
+        move=> dtB.
+        have:= same_ty_det_tree_aux sP sV B ign d.
+        rewrite dtB; case dtB' : det_tree_aux => /=[[DB' blah]|]//=/eqP[?]; subst blah.
+        repeat eexists.
+        destruct d => //=.
+        have [[][//_ ]] := det_tree_aux_func2 dtB.
+        congruence.
+      case nB0: (next_alt _ B0) => [B0'|]//=.
+        case dtA: (det_tree_aux _ _ A) => /=[[DA' sVA]|]//=dtB.
+        have:= same_ty_det_tree_aux sP sV A ign d.
+        rewrite dtA; case dtA' : det_tree_aux => /=[[DA'' blah]|]//=/eqP[?]; subst blah.
+        have:= same_ty_det_tree_aux sP sVA B DA' DA''.
+        rewrite dtB; case dtB' : det_tree_aux => /=[[DB' blah]|]//=/eqP[?]; subst blah.
+        repeat eexists.
+        destruct d => //=.
+        have [[][//_ ]] := det_tree_aux_func2 dtB.
+        destruct DA''; [congruence|].
+        destruct DA'; [|congruence].
+        have [[][//_ ]] := det_tree_aux_func2 dtA.
+        destruct DB'; try congruence.
+      move=> H1.
+      have:= same_ty_det_tree_aux sP sV B d ign.
+      rewrite H1; case dtB' : det_tree_aux => /=[[DB' blah]|]//=/eqP[?]; subst blah.
+      repeat eexists.
+      destruct d => //=.
+      have [[][//]]:= det_tree_aux_func2 H1.
+      congruence.
+Admitted.
+
+(* 
+  Given a checked program, and a deterministic tree,
+  then calling expand produces a tree which is still deterministic.
+*)
+Lemma expand_det_tree1 {u sP sV sV' A r s ign d} : 
+  check_program sP ->
+    sigma2ctx sP s = Some sV ->
+      det_tree_aux sP sV A ign = ty_ok (d, sV') ->
+        expand u s A = r ->
+          exists S d', minD d d' = d' /\ sV_expand sV' S /\
             det_tree_aux sP sV (get_tree r) d = ty_ok (d', S).
 Proof.
   simpl in *.
   rewrite/check_program.
   move=> ckP; elim: A sV sV' r s ign d.
-  - move=> sV1 sV2 r s ign d H [??] <-; subst => /=; repeat eexists; rewrite minD_refl//.
-  - move=> sV1 sV2 r s ign d H [??] <-; subst => /=; repeat eexists; rewrite minD_refl//.
-  - move=> sV1 sV2 r s ign d H [??] <-; subst => /=; repeat eexists; rewrite minD_refl//.
+  - move=> sV1 sV2 r s ign d H [??] <-; subst => /=; repeat eexists; rewrite ?minD_refl//.
+    apply: sV_expand_refl.
+  - move=> sV1 sV2 r s ign d H [??] <-; subst => /=; repeat eexists; rewrite ?minD_refl//.
+    apply: sV_expand_refl.
+  - move=> sV1 sV2 r s ign d H [??] <-; subst => /=; repeat eexists; rewrite ?minD_refl//.
+    apply: sV_expand_refl.
   - admit.
   - move=> sV1 sV2 r s ign d H [??] <-; subst => /=; repeat eexists.
+    apply: sV_expand_refl.
   - move=> A HA s B HB sV1 sV2 r s'/= ign d H.
     case: (ifP (is_dead A)) => DA.
       {
@@ -63,426 +568,15 @@ Proof.
           destruct DA', DB => //=.
           have [[] [//= _ {}H]] := det_tree_aux_func2 dtB.
           rewrite H; congruence.
-        have {HA}/=[S[d'[H1 H2]]]:= HA _ _ _ _ _ _ H dtA e.
+          rewrite/sV_expand => k.
+          case X: lookup => //=[Se].
+          case Y: lookup => //=[Sf|].
+          admit.
+        have {HA}/=[S[d'[H1 [Hx H2]]]]:= HA _ _ _ _ _ _ H dtA e.
         have:= same_ty_det_tree_aux sP sV1 A' DA'(if has_cut A then maxD DA' DB else Pred).
         rewrite H2; case dtA' : det_tree_aux => //=[[Dx Sx]] /eqP[?]; subst Sx.
         have:= same_ty_det_tree_aux sP sV1 B ign (if has_cut A then maxD DA' DB else Pred).
-        rewrite dtB/=; case dtB': det_tree_aux => //=[[Dy Sy]] /eqP[?]; subst Sy.
-        case M1: merge_sig => /=[S'|].
-          repeat eexists.
-          move: dtB' dtA'.
-          case: ifP => cA// {HB}.
-          destruct DA' => //=.
-          destruct DB => //=.
-          rewrite H2 => +[?]; subst.
-          have [[][//_ Hz]] := det_tree_aux_func2 dtB.
-          rewrite Hz => -[?]; subst; rewrite maxD_comm/=.
-          simpl in H1; subst.
-          rewrite (expand_Exp_has_cut _ e)//=.
-        (* BELOW: SHOULD NOT BE REACHABLE: merge_sig S sVB is a ty_ok *)
-        (* sV1 <= sVA
-           sV1 <= sVB
-           sVA + sVB = sV2
-           sV1 <= S 
-           ==========> 
-           goal: merge_sig S sVB = ty_ok
-           IDEA: all vars in S have "compatible" with sVA
-           and all variables not appearing in sVA are also not in sVB, i.e. they are fresh
-
-           FORMALLY:
-            forall x \in S, if x \in sVA, then they are compatible,
-                            else x is not in sVB
-        *)
-        admit.
-      move=> H2.
-      have /=[S[d' [H3 H4]]]  := HA _ _ _ _ _ _ H H2 e.
-      rewrite H4/=.
-      have /= [d1[MM ->]]:= next_alt_None_dt sP sV1 d nB.
-      case: eqP => Hz; repeat eexists; auto.
-    - have fA:= expand_not_failed _ e notF.
-      rewrite next_alt_not_failed//=.
-      move=> + <-{r}/=.
-      rewrite (is_ko_det_tree_aux is_ko_cutr)/=(is_ko_next_alt _ is_ko_cutr)/=.
-      case nB: next_alt => [B'|]//=.
-        case dtA: (det_tree_aux _ _ A) => /=[[DA' sVA]|]//=.
-        case dtB: (det_tree_aux _ _ B) => /=[[DB sVB]|]//=.
-        case M: merge_sig => //=[S']; subst.
-        move=> [??]; subst.
-        have /=[S[d' [H1 H2]]] := HA _ _ _ _ _ _ H dtA e.
-        have := same_ty_det_tree_aux sP sV1 A' DA' (if has_cut A then maxD DA' DB else Pred).
-        rewrite H2/= => /eqP.
-        case Hz : det_tree_aux => //=[[Dx sX]][?]; subst sX.
-        case: eqP; repeat eexists; rewrite //=?minD_refl//=.
-        move: Hz.
-        case:ifP => //= cA.
-        destruct DA'; simpl in *; subst => //.
-        destruct DB => //=; congruence.
-      move=> H2.
-      have /=[S[d' [H0 H1]]]  := HA _ _ _ _ _ _ H H2 e.
-      rewrite H1/=.
-      by case:ifP => //=; repeat eexists; auto; rewrite minD_refl.
-    - have [? fA] := expand_failed_same _ e; subst A'.
-      move=> +<-{r}/=.
-      case nA: next_alt => [A'|]//=; last first.
-        move=> H2.
-        have := same_ty_det_tree_aux sP sV1 B ign d.
-        rewrite H2/=; case H3: det_tree_aux => /=[[D1 Sx]|] => //=/eqP[?]; subst Sx.
-        repeat eexists.
-        destruct d => //=.
-        have [d2[H4 H5]]:= det_tree_aux_func2 H2.
-        destruct d2 => //=.
-        congruence.
-      case nB: next_alt => [B'|]//=; last first.
-        move=> H2.
-        have [d2[H3 H4]]:= det_tree_aux_func2 H2.
-        rewrite minD_comm in H3.
-        destruct d; simpl in H3; subst.
-          by rewrite H4; repeat eexists.
-        move=>/=.
-        have := same_ty_det_tree_aux sP sV1 A ign Pred.
-        by rewrite H2/=; case: det_tree_aux => //= -[]//=; repeat eexists.
-      case dtA: (det_tree_aux _ _ A) => /=[[DA' sVA]|]//=.
-      case dtB: (det_tree_aux _ _ B) => /=[[DB sVB]|]//=.
-      case M: merge_sig => //=[S'][??]; subst.
-      pose X := if has_cut A then maxD DA' DB else Pred.
-      rewrite -/X.
-      have := same_ty_det_tree_aux sP sV1 A ign X.
-      rewrite dtA; case dtA': det_tree_aux => //=[[d' blah]]/eqP[?]; subst blah.
-      have := same_ty_det_tree_aux sP sV1 B ign X.
-      rewrite dtB; case dtB': det_tree_aux => //=[[d1 blah]]/eqP[?]; subst blah.
-      rewrite M/=; repeat eexists.
-      move: dtA' dtB'; rewrite/X.
-      case:ifP => // c.
-      destruct DA' => //=.
-      destruct DB => //=.
-      have [[][//_ ->]] := det_tree_aux_func2 dtA.
-      move=> [?]; subst => /=.
-      have [[][//_ ->]] := det_tree_aux_func2 dtB; congruence.
-    - have [? sA]:= expand_solved_same _ e; subst A'.
-      move=> +<-{r}/=.
-      rewrite next_alt_not_failed?success_failed//=.
-      case nB: next_alt => [B'|]//=; last first.
-        move=> H2; have [d2[H3 H4]] := det_tree_aux_func2 H2.
-        have := same_ty_det_tree_aux sP sV1 A ign d.
-        rewrite H2; case dtA': det_tree_aux => //=[[d' blah]]/eqP[?]; subst blah.
-        repeat eexists; destruct d2; simpl in H3; subst => //.
-        destruct d => //=; congruence.
-      case dtA: (det_tree_aux _ _ A) => /=[[DA' sVA]|]//=.
-      case dtB: (det_tree_aux _ _ B) => /=[[DB sVB]|]//=.
-      case M: merge_sig => //=[S'][??]; subst.
-      have [d2[H2 H3]] := det_tree_aux_func2 dtB.
-      have [d3[H4 H5]]:= det_tree_aux_func2 dtA.
-      pose X := if has_cut A then maxD DA' DB else Pred.
-      rewrite -/X.
-      have := same_ty_det_tree_aux sP sV1 A ign X.
-      rewrite dtA; case dtA': det_tree_aux => //=[[d' blah]]/eqP[?]; subst blah.
-      have := same_ty_det_tree_aux sP sV1 B ign X.
-      rewrite dtB; case dtB': det_tree_aux => //=[[d1 blah]]/eqP[?]; subst blah.
-      rewrite M/=; repeat eexists.
-      move: dtA' dtB'; rewrite/X.
-      case:ifP => // c.
-      destruct DA' => //=.
-      destruct DB => //=.
-      have [[][//_ ->]] := det_tree_aux_func2 dtA.
-      move=> [?]; subst => /=.
-      have [[][//_ ->]] := det_tree_aux_func2 dtB; congruence.
-  - move=> A HA B0 _ B HB sV1 sV2 r s ign d H/=.
-    case e: expand => [A'|A'|A'|A']//=.
-    - have fA:= expand_not_failed _ e notF.
-      have sA:= expand_not_solved_not_success _ e notF.
-      rewrite fA (next_alt_not_failed fA)//= sA/=.
-      move=> + <-{r}/=.
-      case nB0: next_alt => [B0'|]//=.
-        case dtA: (det_tree_aux _ _ A) => /=[[DA' sVA]|]//=.
-        case dtB0: (det_tree_aux _ _ B0) => /=[[DB0 sVB0]|]//=.
-        case dtB: (det_tree_aux _ _ B) => /=[[DB sVB]|]//=.
-        case M: merge_sig => //=[S'][??]; subst.
-        rewrite orbF andbF/=.
-        have {HA}/=[S[d'[H4 H5]]] := HA _ _ _ _ _ _ H dtA e.
-        case nA: next_alt => [A''|]//=; last first.
-          repeat eexists; rewrite minD_refl//.
-        have [d0[//H2 H3]] := det_tree_aux_func2 dtB.
-        case: ifP => fA'.
-          have := same_ty_det_tree_aux sP sV1 A' DA' (maxD DB0 DB).
-          rewrite H5; case dtA': det_tree_aux => //=[[d2 blah]]/eqP[?]; subst blah.
-          (* in S there are more assignemnts than in sV1 *)
-          admit. (*PB WITH SIG*)
-        rewrite orbF.
-        case: ifP.
-          move=> /andP[sA' /eqP nA'].
-          have [dd[//H6 H7]] := next_alt_None_dt sP sV1 (maxD DB0 DB) nA'.
-          rewrite H7/=.
-          case nB: next_alt => [B'|]//=; last first.
-            by repeat eexists; rewrite minD_refl.
-          (* (DEAD \/ (OK /\ ... ! /\ ... OK) \/ Any) /\ B  -> OK /\ B *)
-          admit. (*PB WITH SIG*)
-        have := same_ty_det_tree_aux sP sV1 A' DA' (maxD DB0 DB).
-        rewrite H5; case dtA': det_tree_aux => //=[[d2 blah]]/eqP[?]; subst blah.
-        case sA' : success => //=.
-          move=> {nA A''}.
-          case nA: next_alt => [A''|]//= _.
-          admit. (*PB WITH SIG*)
-        move=> _.
-        admit. (*PB WITH SIG*)
-      case nB: next_alt => [B'|]//=.
-        case dtA: (det_tree_aux _ _ A) => /=[[DA' sVA]|]//=.
-        case dtB0: (det_tree_aux _ _ B0) => /=[[DB0 sVB0]|]//=.
-        case dtB: (det_tree_aux _ _ B) => /=[[DB sVB]|]//=.
-        case M: merge_sig => //=[S'][??]; subst.
-        rewrite orbF andbT.
-        case nA: next_alt => [A''|]//=; last first; rewrite?orbF?orbT/=.
-          repeat eexists; rewrite minD_refl//.
-        rewrite andbT.
-        case: ifP => fA'.
-          repeat eexists; rewrite minD_refl//.
-        rewrite fA'.
-        have [dd[//H2 H3]] := det_tree_aux_func2 dtB.
-        have [d2[H4 H5]] := det_tree_aux_func2 dtA.
-        have {HA}/=[S[d'[H6 H7]]] := HA _ _ _ _ _ _ H dtA e.
-        have := same_ty_det_tree_aux sP sV1 A' DA' (maxD DB0 DB).
-        rewrite H7; case dtA': det_tree_aux => //=[[d3 blah]]/eqP[?]; subst blah.
-        case: ifP => sA'.
-          admit. (*PB WITH SIG*)
-        admit. (*PB WITH SIG*)
-      move=> [??]; subst.
-      rewrite andbT orbT; repeat eexists; rewrite minD_refl//.
-    - have fA:= expand_not_failed _ e notF.
-      have sA:= expand_not_solved_not_success _ e notF.
-      rewrite fA (next_alt_not_failed fA)//= sA/= => +<-{r}/=.
-      case nB0: next_alt => [B0'|]//=.
-        case dtA: (det_tree_aux _ _ A) => /=[[DA' sVA]|]//=.
-        case dtB0: (det_tree_aux _ _ B0) => /=[[DB0 sVB0]|]//=.
-        case dtB: (det_tree_aux _ _ B) => /=[[DB sVB]|]//=.
-        case M: merge_sig => //=[S'][??]; subst.
-        rewrite orbF andbF/=.
-        case nA: next_alt => [A''|]//=; last first.
-          by repeat eexists; rewrite minD_refl.
-        have [xx[//H2 H3]] := det_tree_aux_func2 dtB.
-        have /=[S[d'[H4 H5]]] := HA _ _ _ _ _ _ H dtA e.
-        have := same_ty_det_tree_aux sP sV1 A' DA' (maxD DB0 DB).
-        rewrite H5; case dtA': det_tree_aux => //=[[d2 blah]]/eqP[?]; subst blah.
-        case: ifP => fA'.
-          admit. (*PB WITH SIG*)
-        rewrite orbF/=.
-        case:ifP => H1/=.
-          case:ifP.
-            repeat eexists; rewrite minD_refl//.
-          move=> /eqP nB.
-          admit. (*PB WITH SIG*)
-        admit. (*PB WITH SIG*)
-      rewrite !orbT/=!andbT/=.
-      case nB: next_alt => [B'|]//=; rewrite?orbF ?orbT/=; last first.
-        by move=> [??]; subst; repeat eexists; rewrite minD_refl.
-      case dtA: (det_tree_aux _ _ A) => /=[[DA' sVA]|]//=.
-      case dtB0: (det_tree_aux _ _ B0) => /=[[DB0 sVB0]|]//=.
-      case dtB: (det_tree_aux _ _ B) => /=[[DB sVB]|]//=.
-      case M: merge_sig => //=[S'][??]; subst.
-      case fA': failed => /=.
-        repeat eexists.
-        by rewrite minD_refl.
-      rewrite next_alt_not_failed//=.
-      case:ifP => sA'.
-        admit. (*PB WITH SIG*)
-      have /=[S[d'[H4 H5]]] := HA _ _ _ _ _ _ H dtA e.
-      have := same_ty_det_tree_aux sP sV1 A' DA' (maxD DB0 DB).
-      rewrite H5; case dtA': det_tree_aux => //=[[d2 blah]]/eqP[?]; subst blah.
-      admit. (*PB WITH SIG*)
-    - have [? fA]:= expand_failed_same _ e; subst A' => +<-{r}/=.
-      rewrite fA/=.
-      case:ifP => H1.
-        move=> [??]; subst.
-        by repeat eexists; rewrite minD_refl.
-      case dtA: (det_tree_aux _ _ A) => /=[[DA' sVA]|]//= dtB0.
-      have:= same_ty_det_tree_aux sP sV1 A ign d.
-      rewrite dtA; case dtA' : det_tree_aux => /=[[DA'' blah]|]//=/eqP[?]; subst blah.
-      have:= same_ty_det_tree_aux sP sVA B0 DA' DA''.
-      rewrite dtB0; case dtB0' : det_tree_aux => /=[[DB0'' blah]|]//=/eqP[?]; subst blah.
-      repeat eexists.
-      destruct d => //=.
-      move: H1.
-      case nB0: next_alt => [B0'|]//=; rewrite orbF.
-      case nA: next_alt => [A'|]//= _.
-      have /=[S[d'[H4 H5]]] := HA _ _ _ _ _ _ H dtA e.
-      destruct DA'; destruct DA''; simpl in H4; try congruence.
-      have [[][//_]] := det_tree_aux_func2 dtB0; congruence.
-    - have [? sA]:= expand_solved_same _ e; subst A'.
-      have fA:= success_failed _ sA.
-      rewrite sA fA (next_alt_not_failed fA)/=.
-      case e1: expand => //=[B'|B'|B'|B'].
-      - have fB:= expand_not_failed _ e1 notF.
-        have sB:= expand_not_solved_not_success _ e1 notF.
-        rewrite (next_alt_not_failed fB)//= andbF/=.
-        move=> + <-{r}/=; rewrite fA sA/= (next_alt_not_failed fA)/=.
-        case nA: next_alt => [A'|]//=.
-          case nB0: next_alt => [B0'|]//=.
-            case dtA: (det_tree_aux _ _ A) => /=[[DA' sVA]|]//=.
-            case dtB0: (det_tree_aux _ _ B0) => /=[[DB0 sVB0]|]//=.
-            case dtB: (det_tree_aux _ _ B) => /=[[DB sVB]|]//=.
-            case M: merge_sig => //=[S'][??]; subst.
-            have := same_ty_det_tree_aux sP sV1 A ign (maxD DB0 DB).
-            rewrite dtA; case dtA': det_tree_aux => //=[[d2 blah]]/eqP[?]; subst blah.
-            
-            have := same_ty_det_tree_aux sP sVA B0 DA' d2.
-            rewrite dtB0; case dtB0': det_tree_aux => //=[[d3 blah]]/eqP[?]; subst blah.
-
-            have /= := HB _ _ _ _ _ _ _ dtB e1.
-            (*PB WITH IH*)
-            admit.
-          move=> dtB.
-          case nB: next_alt => [B''|]//=.
-            apply: HB _ _ _ _ _ _ dtB e1.
-            admit. (*PB WITH IH*)
-          repeat eexists; rewrite minD_refl//.
-        case nB0: next_alt => [B0'|]//=.
-          case dtA: (det_tree_aux _ _ A) => /=[[DA' sVA]|]//=dtB.
-          have := same_ty_det_tree_aux sP sV1 A ign d.
-          rewrite dtA; case dtA': det_tree_aux => //=[[d2 blah]]/eqP[?]; subst blah.
-          case:eqP => nB'.
-            by repeat eexists; rewrite minD_refl.
-          admit.
-        move=> dtB.
-        case nB: next_alt => [B''|]//=.
-          apply: HB dtB e1.
-          admit.
-        repeat eexists; rewrite minD_refl//.
-      - have fB:= expand_not_failed _ e1 notF.
-        have sB:= expand_not_solved_not_success _ e1 notF.
-        rewrite (next_alt_not_failed fB)//= andbF/=.
-        move=> + <-{r}/=.
-        rewrite (is_ko_next_alt _ is_ko_cutr)/=.
-        rewrite failed_success_cut success_cut sA/=next_alt_cutl/=.
-        rewrite (@next_alt_not_failed (cutl A))/=; last first.
-          rewrite failed_success_cut success_cut sA//.
-        case nA: next_alt => [A'|]//=.
-          case nB0: next_alt => [B0'|]//=.
-            case dtA: (det_tree_aux _ _ A) => /=[[DA' sVA]|]//=.
-            case dtB0: (det_tree_aux _ _ B0) => /=[[DB0 sVB0]|]//=.
-            case dtB: (det_tree_aux _ _ B) => /=[[DB sVB]|]//=.
-            case M: merge_sig => //=[S'][??]; subst.
-            case: eqP => nB'.
-              by repeat eexists; rewrite minD_refl//.
-            admit.
-          move=> H1.
-          case nB: next_alt => [B''|]/=; last first.
-            by repeat eexists; rewrite minD_refl.
-          apply: HB _ _ _ _ _ _ H1 e1.
-          admit.
-        case nB0: next_alt => [B0'|]//=.
-          case dtA: (det_tree_aux _ _ A) => /=[[DA' sVA]|]//=.
-          case dtB: (det_tree_aux _ _ B) => /=[[DB sVB]|]//=[??]; subst.
-          case nB: next_alt => [B''|]/=; last first.
-            by repeat eexists; rewrite minD_refl.
-          have [d1[H1]] := next_alt_None_dt sP sV1 ign nA.
-          rewrite dtA => -[??]; subst.
-          apply: HB dtB e1.
-          admit.
-        move=> dtB.
-        case nB: next_alt => [B''|]/=; last first.
-          by repeat eexists; rewrite minD_refl.
-        apply: HB dtB e1.
-        admit.
-      - have [? fB]:= expand_failed_same _ e1; subst B' => +<-{r}/=.
-        rewrite fA/=sA (next_alt_not_failed fA)/=.
-        case nB0: (next_alt _ B0) => [B0'|]//=.
-          rewrite orbF/=.
-          case nA: next_alt => [A'|]//=.
-            case dtA: (det_tree_aux _ _ A) => /=[[DA' sVA]|]//=.
-            case dtB0: (det_tree_aux _ _ B0) => /=[[DB0 sVB0]|]//=.
-            case dtB: (det_tree_aux _ _ B) => /=[[DB sVB]|]//=.
-            case M: merge_sig => //=[S'][??]; subst.
-            have := same_ty_det_tree_aux sP sV1 A ign (maxD DB0 DB).
-            rewrite dtA; case dtA': det_tree_aux => //=[[d2 blah]]/eqP[?]; subst blah.
-            have := same_ty_det_tree_aux sP sVA B DA' d2.
-            rewrite dtB; case dtB': det_tree_aux => //=[[d3 blah]]/eqP[?]; subst blah.
-            have := same_ty_det_tree_aux sP sVA B0 DA' d2.
-            rewrite dtB0; case dtB0': det_tree_aux => //=[[d4 blah]]/eqP[?]; subst blah.
-            rewrite M/=.
-            repeat eexists.
-            destruct DB0, DB => //=; simpl in *.
-            have /=[Sx [d'[H1 H2]]] := HA _ _ _ _ _ _ H dtA e.
-            admit.
-          case nB: next_alt => [B''|]//=.
-            case dtA: (det_tree_aux _ _ A) => /=[[DA' sVA]|]//=.
-            move=>dtB.
-            have := same_ty_det_tree_aux sP sV1 A ign d.
-            rewrite dtA; case dtA': det_tree_aux => //=[[d2 blah]]/eqP[?]; subst blah.
-            have := same_ty_det_tree_aux sP sVA B DA' d2.
-            rewrite dtB; case dtB': det_tree_aux => //=[[d3 blah]]/eqP[?]; subst blah.
-            repeat eexists.
-            have /=[Sx [d'[H1 H2]]] := HA _ _ _ _ _ _ H dtA e.
-            destruct d => //=.
-            admit.
-          move=> [??]; subst.
-          by repeat eexists; rewrite minD_refl.
-        case nB: next_alt => [B'|]//=; last first.
-          move=> [??]; subst.
-          by repeat eexists; rewrite minD_refl.
-        rewrite orbT/= => dtB.
-        have:= same_ty_det_tree_aux sP sV1 B ign d.
-        rewrite dtB; case dtB' : det_tree_aux => /=[[DB' blah]|]//=/eqP[?]; subst blah.
-        repeat eexists.
-        destruct d => //=.
-        have [[][//_ ]] := det_tree_aux_func2 dtB.
-        congruence.
-      - have [? sB]:= expand_solved_same _ e1; subst B'.
-        have fB:= success_failed _ sB.
-        move=> +<-{r}/=; rewrite fA sA /=.
-        rewrite (next_alt_not_failed fB) andbF/=.
-        rewrite (next_alt_not_failed fA)/=.
-        case nA: next_alt => [A'|]//=.
-          case nB0: (next_alt _ B0) => [B0'|]//=.
-            case dtA: (det_tree_aux _ _ A) => /=[[DA' sVA]|]//=.
-            case dtB0: (det_tree_aux _ _ B0) => /=[[DB0 sVB0]|]//=.
-            case dtB: (det_tree_aux _ _ B) => /=[[DB sVB]|]//=.
-            case M: merge_sig => //=[S'][??]; subst.
-            have /=[Sx [d'[H1 H2]]] := HA _ _ _ _ _ _ H dtA e.
-            (* have /= := HB _ _ _ _ _ _ _ dtB e1. *)
-            have:= same_ty_det_tree_aux sP sV1 A ign (maxD DB0 DB).
-            rewrite dtA; case dtA' : det_tree_aux => /=[[DA'' blah]|]//=/eqP[?]; subst blah.
-            have:= same_ty_det_tree_aux sP sVA B0 DA' DA''.
-            rewrite dtB0; case dtB0' : det_tree_aux => /=[[DB0'' blah]|]//=/eqP[?]; subst blah.
-            have:= same_ty_det_tree_aux sP sVA B DA' DA''.
-            rewrite dtB; case dtB' : det_tree_aux => /=[[DB'' blah]|]//=/eqP[?]; subst blah.
-            rewrite M/=.
-            repeat eexists.
-            destruct DB0 => //=.
-            destruct DB => //=.
-            simpl in *.
-            have [[][//_ H3]] := det_tree_aux_func2 dtB0.
-            have [[][//_ H4]] := det_tree_aux_func2 dtB.
-            destruct DA''.
-              have->/=: DB0'' = Func by congruence.
-              by have->/=: DB'' = Func by congruence.
-            destruct DA'; simpl in H1; subst => //=; try congruence.
-            admit. (*PB with max DB0 DB*)
-          move=> dtB.
-          have:= same_ty_det_tree_aux sP sV1 B ign d.
-          rewrite dtB; case dtB' : det_tree_aux => /=[[DB' blah]|]//=/eqP[?]; subst blah.
-          repeat eexists.
-          destruct d => //=.
-          have [[][//_ ]] := det_tree_aux_func2 dtB.
-          congruence.
-        case nB0: (next_alt _ B0) => [B0'|]//=.
-          case dtA: (det_tree_aux _ _ A) => /=[[DA' sVA]|]//=dtB.
-          have:= same_ty_det_tree_aux sP sV1 A ign d.
-          rewrite dtA; case dtA' : det_tree_aux => /=[[DA'' blah]|]//=/eqP[?]; subst blah.
-          have:= same_ty_det_tree_aux sP sVA B DA' DA''.
-          rewrite dtB; case dtB' : det_tree_aux => /=[[DB' blah]|]//=/eqP[?]; subst blah.
-          repeat eexists.
-          destruct d => //=.
-          have [[][//_ ]] := det_tree_aux_func2 dtB.
-          destruct DA''; [congruence|].
-          destruct DA'; [|congruence].
-          have [[][//_ ]] := det_tree_aux_func2 dtA.
-          destruct DB'; try congruence.
-        move=> H1.
-        have:= same_ty_det_tree_aux sP sV1 B d ign.
-        rewrite H1; case dtB' : det_tree_aux => /=[[DB' blah]|]//=/eqP[?]; subst blah.
-        repeat eexists.
-        destruct d => //=.
-        have [[][//]]:= det_tree_aux_func2 H1.
-        congruence.
-Admitted.
+Abort.
 
 Definition is_det s A := forall u s' B n,
   runb u s A s' B n -> next_alt false B = None.
